

2 layer MLP

FF

$$\text{net}^1 = w^1 * x^T$$

$$o^1 = f^1(\text{net}^1) = \text{Sigmoid}(\text{net}^1)$$

$$\text{net}^2 = w^2 * o^1$$

$$o^2 = f^2(\text{net}^2) = \text{net}^2$$

BP

$$w^2 = w^2 - \eta \left(\frac{\partial E}{\partial e} \frac{\partial e}{\partial o^2} \frac{\partial o^2}{\partial \text{net}^2} \frac{\partial \text{net}^2}{\partial w^2} \right)$$

$$e \quad -1 \quad 1 \quad o^1$$

$$w^1 = w^1 - \eta \left(\frac{\partial E}{\partial e} \frac{\partial e}{\partial o^2} \frac{\partial o^2}{\partial \text{net}^2} \frac{\partial \text{net}^2}{\partial o^1} \frac{\partial o^1}{\partial \text{net}^1} \frac{\partial \text{net}^1}{\partial w^1} \right)$$

$$e \quad -1 \quad 1 \quad w^2 \quad f'^1 \quad x^T$$

3 layer MLP

FF

$$\text{net}^1 = w^1 + x^T$$

$$o^1 = f'(\text{net}^1) = \text{Sigmoid}(\text{net}^1)$$

$$\text{net}^2 = w^2 + o^1$$

$$o^2 = f'(\text{net}^2) = \text{Sigmoid}(\text{net}^2)$$

$$\text{net}^3 = w^3 + o^2$$

$$o^3 = f'(\text{net}^3) = \text{net}^3$$

BP

$$w^3 = w^3 - \eta \left(\frac{\partial E}{\partial e} \frac{\partial e}{\partial o^3} \frac{\partial o^3}{\partial \text{net}^3} \frac{\partial \text{net}^3}{\partial w^3} \right)$$

$$e \quad -1 \quad 1 \quad o^2$$

$$w^2 = w^2 - \eta \left(\frac{\partial E}{\partial e} \frac{\partial e}{\partial o^3} \frac{\partial o^3}{\partial \text{net}^3} \frac{\partial \text{net}^3}{\partial o^2} \frac{\partial o^2}{\partial \text{net}^2} \frac{\partial \text{net}^2}{\partial w^2} \right)$$

$$e \quad -1 \quad 1 \quad w^3 \quad f'^2 \quad o^1$$

$$w^1 = w^1 - \eta \left(\frac{\partial E}{\partial e} \frac{\partial e}{\partial o^3} \frac{\partial o^3}{\partial \text{net}^3} \frac{\partial \text{net}^3}{\partial o^2} \frac{\partial o^2}{\partial \text{net}^2} \frac{\partial \text{net}^2}{\partial o^1} \frac{\partial o^1}{\partial \text{net}^1} \frac{\partial \text{net}^1}{\partial w^1} \right)$$

$$e \quad -1 \quad 1 \quad w^3 \quad f'^2 \quad w^2 \quad f'^1 \quad x^T$$

3 layer AE + 2 layer MLP + Global Train

FF

$$\text{net}^{e1} = w^{e1} \times x^T$$

$$h^1 = f^{e1}(\text{net}^{e1}) = \text{Sigmoid}(\text{net}^{e1})$$

$$\text{net}^{e2} = w^{e2} \times h^1$$

$$h^2 = f^{e2}(\text{net}^{e2}) = \text{Sigmoid}(\text{net}^{e2})$$

$$\text{net}^{e3} = w^{e3} \times h^2$$

$$h^3 = f^{e3}(\text{net}^{e3}) = \text{Sigmoid}(\text{net}^{e3})$$

$$\text{net}^1 = w^1 \times h^3$$

$$o^1 = f^1(\text{net}^1) = \text{Sigmoid}(\text{net}^1)$$

$$\text{net}^2 = w^2 \times o^1$$

$$o^2 = f^2(\text{net}^2) = \text{net}^2$$

BP

$$w^{e1} = w^{e1} - \eta \left(\frac{\partial E}{\partial e} \frac{\partial e}{\partial o^2} \frac{\partial o^2}{\partial \text{net}^2} \frac{\partial \text{net}^2}{\partial o^1} \frac{\partial o^1}{\partial \text{net}^1} \frac{\partial \text{net}^1}{\partial h^3} \frac{\partial h^3}{\partial \text{net}^{e3}} \frac{\partial \text{net}^{e3}}{\partial h^2} \frac{\partial h^2}{\partial \text{net}^{e2}} \frac{\partial \text{net}^{e2}}{\partial h^1} \frac{\partial h^1}{\partial \text{net}^{e1}} \frac{\partial \text{net}^{e1}}{\partial w^{e1}} \right)$$

$$e \quad -1 \quad 1 \quad w^2 \quad f'^1 \quad w^1 \quad f'^{e3} \quad w^{e3} \quad f'^{e2} \quad w^{e2} \quad f'^{e1} \quad \times$$

$$w^{e2} = w^{e2} - \eta \left(\frac{\partial E}{\partial e} \frac{\partial e}{\partial o^2} \frac{\partial o^2}{\partial \text{net}^2} \frac{\partial \text{net}^2}{\partial o^1} \frac{\partial o^1}{\partial \text{net}^1} \frac{\partial \text{net}^1}{\partial h^3} \frac{\partial h^3}{\partial \text{net}^{e3}} \frac{\partial \text{net}^{e3}}{\partial h^2} \frac{\partial h^2}{\partial \text{net}^{e2}} \frac{\partial \text{net}^{e2}}{\partial w^{e2}} \right)$$

$$e \quad -1 \quad 1 \quad w^2 \quad f'^1 \quad w^1 \quad f'^{e3} \quad w^{e3} \quad f'^{e2} \quad h^1$$

$$w^{e3} = w^{e3} - \eta \left(\frac{\partial E}{\partial e} \frac{\partial e}{\partial o^2} \frac{\partial o^2}{\partial \text{net}^2} \frac{\partial \text{net}^2}{\partial o^1} \frac{\partial o^1}{\partial \text{net}^1} \frac{\partial \text{net}^1}{\partial h^3} \frac{\partial h^3}{\partial \text{net}^{e3}} \frac{\partial \text{net}^{e3}}{\partial w^{e3}} \right)$$

$$e \quad -1 \quad 1 \quad w^2 \quad f'^1 \quad w^1 \quad f'^{e3} \quad h^2$$

$$w^1 = w^1 - \eta \left(\frac{\partial E}{\partial e} \frac{\partial e}{\partial o^2} \frac{\partial o^2}{\partial \text{net}^2} \frac{\partial \text{net}^2}{\partial o^1} \frac{\partial o^1}{\partial \text{net}^1} \frac{\partial \text{net}^1}{\partial w^1} \right)$$

$$e \quad -1 \quad 1 \quad w^2 \quad f'^1 \quad h^3$$

$$w^2 = w^2 - \eta \left(\frac{\partial E}{\partial e} \frac{\partial e}{\partial o^2} \frac{\partial o^2}{\partial \text{net}^2} \frac{\partial \text{net}^2}{\partial w^2} \right)$$

$$e \quad -1 \quad 1 \quad o^1$$

3 layer AE + 3 layer MLP + Global Train

FF

$$\text{net}^{e1} = w^{e1} * x^T$$

$$h^1 = f^{e1}(\text{net}^{e1}) = \text{Sigmoid}(\text{net}^{e1})$$

$$\text{net}^{e2} = w^{e2} * h^1$$

$$h^2 = f^{e2}(\text{net}^{e2}) = \text{Sigmoid}(\text{net}^{e2})$$

$$\text{net}^{e3} = w^{e3} * h^2$$

$$h^3 = f^{e3}(\text{net}^{e3}) = \text{Sigmoid}(\text{net}^{e3})$$

$$\text{net}^1 = w^1 * h^3$$

$$o^1 = f^1(\text{net}^1) = \text{Sigmoid}(\text{net}^1)$$

$$\text{net}^2 = w^2 * o^1$$

$$o^2 = f^2(\text{net}^2) = \text{Sigmoid}(\text{net}^2)$$

$$\text{net}^3 = w^3 * o^2$$

$$o^3 = f^3(\text{net}^3) = \text{net}^3$$

BP

$$w^{e1} = w^{e1} - \eta \left(\frac{\partial E}{\partial e} \frac{\partial e}{\partial o^3} \frac{\partial o^3}{\partial \text{net}^3} \frac{\partial \text{net}^3}{\partial o^2} \frac{\partial o^2}{\partial \text{net}^2} \frac{\partial \text{net}^2}{\partial o^1} \frac{\partial o^1}{\partial \text{net}^1} \frac{\partial \text{net}^1}{\partial h^3} \frac{\partial h^3}{\partial \text{net}^{e3}} \frac{\partial \text{net}^{e3}}{\partial h^2} \right)$$

$$\left(\frac{\partial h^2}{\partial \text{net}^{e2}} \frac{\partial \text{net}^{e2}}{\partial h^1} \frac{\partial h^1}{\partial \text{net}^{e1}} \frac{\partial \text{net}^{e1}}{\partial w^{e1}} \right)$$

$$w^{e2} = w^{e2} - \eta \left(\frac{\partial E}{\partial e} \frac{\partial e}{\partial o^3} \frac{\partial o^3}{\partial \text{net}^3} \frac{\partial \text{net}^3}{\partial o^2} \frac{\partial o^2}{\partial \text{net}^2} \frac{\partial \text{net}^2}{\partial o^1} \frac{\partial o^1}{\partial \text{net}^1} \frac{\partial \text{net}^1}{\partial h^3} \frac{\partial h^3}{\partial \text{net}^{e3}} \frac{\partial \text{net}^{e3}}{\partial h^2} \frac{\partial h^2}{\partial \text{net}^{e2}} \right)$$

$$w^{e3} = w^{e3} - \eta \left(\frac{\partial E}{\partial e} \frac{\partial e}{\partial o^3} \frac{\partial o^3}{\partial \text{net}^3} \frac{\partial \text{net}^3}{\partial o^2} \frac{\partial o^2}{\partial \text{net}^2} \frac{\partial \text{net}^2}{\partial o^1} \frac{\partial o^1}{\partial \text{net}^1} \frac{\partial \text{net}^1}{\partial h^3} \frac{\partial h^3}{\partial \text{net}^{e3}} \frac{\partial \text{net}^{e3}}{\partial w^{e3}} \right)$$

$$w^1 = w^1 - \eta \left(\frac{\partial E}{\partial e} \frac{\partial e}{\partial o^3} \frac{\partial o^3}{\partial \text{net}^3} \frac{\partial \text{net}^3}{\partial o^2} \frac{\partial o^2}{\partial \text{net}^2} \frac{\partial \text{net}^2}{\partial o^1} \frac{\partial o^1}{\partial \text{net}^1} \frac{\partial \text{net}^1}{\partial w^1} \right)$$

$$w^2 = w^2 - \eta \left(\frac{\partial E}{\partial e} \frac{\partial e}{\partial o^3} \frac{\partial o^3}{\partial \text{net}^3} \frac{\partial \text{net}^3}{\partial o^2} \frac{\partial o^2}{\partial \text{net}^2} \frac{\partial \text{net}^2}{\partial w^2} \right)$$

$$w^3 = w^3 - \eta \left(\frac{\partial E}{\partial e} \frac{\partial e}{\partial o^3} \frac{\partial o^3}{\partial \text{net}^3} \frac{\partial \text{net}^3}{\partial w^3} \right)$$